term.fst
@@ -100,7 +100,7 @@ let rec is_var_present v t =
   and is_var_present_list v term_list =
   match term_list with
   | [] -> true
-  | hd::tl -> (is_var_present v hd) && (is_var_present_list v tl)
+  | hd::tl -> (is_var_present v hd) || (is_var_present_list v tl)
 
 
 
